Superposition_Calculus/First_Order_Superposition_Example.thy
@@ -19,6 +19,7 @@ interpretation first_order_superposition_calculus
   "trivial_select :: ('f :: weighted, 'v :: infinite) select" 
   less_kbo
   trivial_tiebreakers
+  "\<lambda>_. ([], ())"
 proof(unfold_locales)
   fix clause :: "('f, 'v) atom clause"
 
